Almost complete re-write of label-free language

label-free/Semantics.v
@@ -1,51 +1,66 @@
+(* TODO: imports are messed up now that there's a module *) 
 Require Import Syntax.
 Require Import Substitution.
 Require Import LibList.
 Require Import LibListSorted.
-Require Import LibRelation.
+Require Import Arith.
 
 Open Scope label_free_is5_scope.
 
 Global Reserved Notation " G '|=' Gamma '|-' M ':::' A " (at level 70).
 
-Definition Context_LF := list ty_LF.
 Definition Background_LF := list Context_LF.
 
 (* Statics *)
+
 Inductive types_LF: Background_LF -> Context_LF -> te_LF -> ty_LF -> Prop :=
+
 | t_hyp_LF: forall A G Gamma v_n
-  (HT: nth_error Gamma v_n = Some A),
+  (HT: Nth v_n Gamma A),
   G |= Gamma |- (hyp_LF v_n) ::: A
+
 | t_lam_LF: forall A B G Gamma M 
   (HT: G |= A::Gamma |- M ::: B),
   G |= Gamma |- (lam_LF A M) ::: A ---> B
+
 | t_appl_LF: forall A B G Gamma M N
   (HT1: G |= Gamma |- M ::: A ---> B)
   (HT2: G |= Gamma |- N ::: A),
   G |= Gamma |- (appl_LF M N) ::: B
+
 | t_box_LF: forall A G Gamma M
   (HT: G & Gamma |= nil |- M ::: A),
   G |= Gamma |- (box_LF M) ::: [*] A
+
 | t_unbox_LF: forall A G Gamma M
   (HT: G |= Gamma |- M ::: [*] A),
   G |= Gamma |- unbox_LF M ::: A
+
 | t_unbox_fetch_LF: forall A G Gamma Gamma' M
   (HT: G & Gamma' |= Gamma |- M ::: [*] A),
-  forall G0, permut (G & Gamma) G0 -> G0 |= Gamma' |- unbox_fetch_LF M ::: A
+  forall G', permut (G & Gamma) G' ->
+    G' |= Gamma' |- unbox_fetch_LF M Gamma ::: A
+
 | t_here_LF: forall A G Gamma M
   (HT: G |= Gamma |- M ::: A),
   G |= Gamma |- here_LF M ::: <*> A
+
 | t_get_here_LF: forall A G Gamma Gamma' M
   (HT: G & Gamma' |= Gamma |- M ::: A),
-  forall G0, permut (G & Gamma) G0 -> G0 |= Gamma' |- get_here_LF M ::: <*> A
+  forall G0, permut (G & Gamma) G0 -> 
+    G0 |= Gamma' |- get_here_LF M Gamma ::: <*> A
+
 | t_letdia_LF: forall A B G Gamma M N
   (HT1: G |= Gamma |- M ::: <*> A)
   (HT2: (A :: nil) :: G |= Gamma |- N ::: B),
   G |= Gamma |- letdia_LF M N ::: B 
+
 | t_letdia_get_LF: forall A B G Gamma Gamma' M N
   (HT1: G & Gamma' |= Gamma |- M ::: <*> A)
   (HT2: (A :: nil) :: G & Gamma |= Gamma' |- N ::: B),
-  forall G0, permut (G & Gamma) G0 -> G0 |= Gamma' |- letdia_get_LF M N ::: B
+  forall G0, permut (G & Gamma) G0 -> 
+    G0 |= Gamma' |- letdia_get_LF M N Gamma ::: B
+
 where " G '|=' Gamma '|-' M ':::' A " := (types_LF G Gamma M A) : label_free_is5_scope.
 
 (* Dynamics *)
@@ -54,42 +69,99 @@ Inductive value_LF: te_LF -> Prop :=
 | val_lam_LF: forall A M, value_LF (lam_LF A M)
 | val_box_LF: forall M, value_LF (box_LF M)
 | val_here_LF: forall M, value_LF M -> value_LF (here_LF M)
-| val_get_here_LF: forall M, value_LF M -> value_LF (get_here_LF M)
+| val_get_here_LF: forall M Gamma, value_LF M -> value_LF (get_here_LF M Gamma)
 .
 
 Global Reserved Notation " M |-> N " (at level 70).
 
-Inductive step_LF: te_LF -> te_LF -> Prop :=
-| red_appl_lam_LF: forall M A N, appl_LF (lam_LF A M) N |-> [N//0] M
-| red_unbox_box_LF: forall M, unbox_LF (box_LF M) |-> M
-| red_unbox_fetch_box_LF: forall M, unbox_fetch_LF (box_LF M) |-> M
-| red_letdia_here_LF: forall M N, letdia_LF (here_LF M) N |-> [M//0]N
-| red_letdia__get_here_LF: forall M N, letdia_LF (get_here_LF M) N |-> [M//0]N
-| red_letdia_get__here_LF: forall M N, letdia_get_LF (here_LF M) N |-> [M//0]N
-| red_letdia_get_get_here_LF: forall M N, letdia_get_LF (get_here_LF M) N |-> [M//0]N
-| red_appl_LF: forall M N M' (HT: M |-> M'), appl_LF M N |-> appl_LF M' N
-| red_unbox_LF: forall M M' (HT: M |-> M'), unbox_LF M |-> unbox_LF M'
-| red_unbox_fetch_LF: forall M M' (HT: M |-> M'), unbox_fetch_LF M |-> unbox_fetch_LF M'
-| red_dia_here_LF: forall M M' (HT: M |-> M'), here_LF M |-> here_LF M'
-| red_dia_move_LF: forall M M' (HT: M |-> M'), get_here_LF M |-> get_here_LF M'
-| red_letdia_LF: forall M N M' (HT: M |-> M'), letdia_LF M N |-> letdia_LF M' N
-| red_letdia_move_LF: forall M N M' (HT: M |-> M'), letdia_get_LF M N |-> letdia_get_LF M' N
+Inductive step_LF: (te_LF * Context_LF * Background_LF) -> (te_LF * Context_LF * Background_LF) -> Prop :=
+
+| red_appl_lam_LF: forall G Gamma M A N,
+  (appl_LF (lam_LF A M) N, Gamma, G) |-> 
+    ([N//0 | Gamma][M | Gamma], Gamma, G)
+
+| red_unbox_box_LF: forall G Gamma M, (* ! ?added nil to G ! *)
+  (unbox_LF (box_LF M), Gamma, G) |-> 
+    (M, Gamma, G)
+
+| red_unbox_fetch_box_LF: forall G Gamma Gamma' M, (* ! ?added nil to G ! *)
+  (unbox_fetch_LF (box_LF M) Gamma', Gamma, G) |-> 
+    (M, Gamma, G) 
+
+| red_letdia_here_LF: forall G Gamma M N A,
+  G |= Gamma |- here_LF M ::: <*>A ->
+  (letdia_LF (here_LF M) N, Gamma, G) |-> 
+    ([M // 0 | (A::nil)][N | Gamma], Gamma, G)
+
+| red_letdia__get_here_LF: forall G Gamma Gamma' M N A,
+  G |= Gamma |- get_here_LF M Gamma' ::: <*> A ->
+  (letdia_LF (get_here_LF M Gamma') N, Gamma, G) |-> 
+    ([M // 0 | (A::nil)][N | Gamma] , Gamma, G)
+
+| red_letdia_get__here_LF: forall G G' Gamma Gamma' M N A,
+  permut (G' & Gamma') (G & Gamma) ->
+  G' |= Gamma' |- here_LF M ::: <*> A ->
+  (letdia_get_LF (here_LF M) N Gamma', Gamma, G) |-> 
+    ([M // 0 | (A::nil)][N | Gamma], Gamma, G)
+
+| red_letdia_get_get_here_LF: forall G G' Gamma Gamma' Delta M N A,
+  permut (G' & Gamma') (G & Gamma) ->
+  G' |= Gamma' |- get_here_LF M Delta ::: <*> A ->
+  (letdia_get_LF (get_here_LF M Delta) N Gamma', Gamma, G) |-> 
+    ([M // 0 | (A::nil)][N | Gamma], Gamma, G)
+
+| red_appl_LF: forall G Gamma M N M'
+  (HT: (M, Gamma, G) |-> (M', Gamma, G)), 
+  (appl_LF M N, Gamma, G) |-> (appl_LF M' N, Gamma, G)
+
+| red_unbox_LF: forall G Gamma M M'
+  (HT: (M, Gamma, G) |-> (M', Gamma, G)), 
+  (unbox_LF M, Gamma, G) |-> (unbox_LF M', Gamma, G)
+
+| red_unbox_fetch_LF: forall G G' Gamma' M M' Gamma
+(*
+  (HPermutG': permut G' (G & Gamma'))
+  (HPermutG'': permut G'' (G & Gamma))
+*)
+  (HT: (M, Gamma', G') |-> (M', Gamma', G')), 
+  (unbox_fetch_LF M Gamma', Gamma, G) |-> (unbox_fetch_LF M' Gamma', Gamma, G)
+
+| red_here_LF: forall G Gamma M M' 
+  (HT: (M, Gamma, G) |-> (M', Gamma, G)), 
+  (here_LF M, Gamma, G) |-> (here_LF M', Gamma, G)
+
+| red_get_here_LF: forall G  G' Gamma Gamma' M M' 
+(*
+  (HPermutG': permut G' (G & Gamma'))
+  (HPermutG'': permut G'' (G & Gamma))
+*)
+  (HT: (M, Gamma, G') |-> (M', Gamma, G')), 
+  (get_here_LF M Gamma, Gamma', G) |-> (get_here_LF M' Gamma, Gamma', G)
+
+| red_letdia_LF: forall G Gamma M N M' 
+  (HT: (M, Gamma, G) |-> (M', Gamma, G)),
+  (letdia_LF M N, Gamma, G) |-> (letdia_LF M' N, Gamma, G)
+
+| red_letdia_move_LF: forall G G' Gamma Gamma' M N M'
+(*
+  (HPermutG': permut G' (G & Gamma'))
+  (HPermutG'': permut G'' (G & Gamma)) 
+*)
+  (HT: (M, Gamma, G') |-> (M', Gamma, G')), 
+  (letdia_get_LF M N Gamma, Gamma', G) |-> (letdia_get_LF M' N Gamma, Gamma', G)
+
 where " M |-> N " := (step_LF M N ) : label_free_is5_scope.
 
 Section Lemmas.
-
-Lemma eq_context_dec:
-forall Gamma Gamma': Context_LF, {Gamma = Gamma'} + {Gamma <> Gamma'}.
-  intros; decide equality; decide equality.
-Qed.
 
 (* TODO: this may be moved to a separate file *)
 (* Permutation *)
 
 (* TODO *)
 Lemma PermutLastSame:
-forall A G G' (elem:A)
-  (HT: permut (G & elem) (G' & elem)),
+forall A G G' (elem:A),
+  permut (G & elem) (G' & elem)
+  <->
   permut G G'.
 Admitted.
 
@@ -120,7 +192,7 @@ destruct HSubst as [GT];
 apply t_unbox_fetch_LF with (Gamma:=Gamma) (G:=G++GT).
 apply IHHT;
   exists GT; permut_simpl.
-apply permut_trans with (l2:= G0 ++ GT); 
+apply permut_trans with (l2:= G' ++ GT); 
 [ permut_simpl | ]; assumption.
 (* get_here *)
 destruct HSubst as [GT];
@@ -154,25 +226,88 @@ apply BackgroundSubsetImpl with (G:=G++G');
 [assumption | exists (Ctx::nil); permut_simpl].
 Qed.
 
+(* When we have e.g. unbox_fetch M' Gamma and we weaken Gamma into Gamma++Delta, 
+   we need to change the term as well *)
+
+Reserved Notation " {{ A ~> B }} M " (at level 70).  
+Reserved Notation " }} A ~> B {{ [ M | C ] " (at level 70).
+
+Fixpoint inner_term_weakening (M: te_LF) (Gamma: Context_LF) (Delta: Context_LF) :=
+match M with
+| hyp_LF n => hyp_LF n
+| lam_LF A M' => lam_LF A ({{ Delta ~> A::Gamma}} M')
+| appl_LF M' N => appl_LF ({{Delta ~> Gamma}} M') ({{Delta ~> Gamma}} N)
+| box_LF M' => box_LF (}}Delta ~> Gamma{{ [ M' | nil ] )
+| unbox_LF M' => unbox_LF ({{Delta ~> Gamma}} M')
+| unbox_fetch_LF M' Gamma' => unbox_fetch_LF (}}Delta ~> Gamma{{ [M' | Gamma']) Gamma'
+| here_LF M' => here_LF ({{Delta ~> Gamma}} M') 
+| get_here_LF M' Gamma' => get_here_LF (}}Delta ~> Gamma{{ [M' | Gamma']) Gamma'
+| letdia_LF M' N => letdia_LF ({{Delta ~> Gamma}} M') ({{Delta ~> Gamma}} N)
+| letdia_get_LF M' N Gamma' =>
+  letdia_get_LF (}}Delta ~> Gamma{{ [M' | Gamma']) ({{Delta ~> Gamma}} N) Gamma'
+end
+where " {{ A ~> B }} M " := (inner_term_weakening M B A)
+with
+outer_term_weakening  (M: te_LF) (Gamma: Context_LF) (Gamma': Context_LF) (Delta: Context_LF) :=
+match M with
+| hyp_LF n => hyp_LF n
+| lam_LF A M' => lam_LF A (}}Delta ~> Gamma'{{ [M'| A::Gamma])
+| appl_LF M' N => 
+  appl_LF (}} Delta ~> Gamma'{{ [M'| Gamma]) (}}Delta ~> Gamma'{{ [N | Gamma])
+| box_LF M' => box_LF (}} Delta ~> Gamma'{{ [M' | nil])
+(*
+  match eq_context_LF_dec Gamma' nil with
+    | left _ => box_LF ({{Delta ~> nil}} M')
+    | right _ => box_LF (}}Delta ~> Gamma'{{ [M' | nil])
+  end
+*)
+| unbox_LF M' => unbox_LF (}}Delta ~> Gamma'{{ [M' | Gamma])
+| unbox_fetch_LF M' Gamma'' =>
+  match eq_context_LF_dec Gamma' Gamma'' with
+    | left _ => unbox_fetch_LF ({{Delta ~> Gamma''}} M') (Gamma''++Delta)
+    | right _ => unbox_fetch_LF (}}Delta ~> Gamma'{{ [M' | Gamma'']) Gamma''
+  end
+| here_LF M' => here_LF (}}Delta ~> Gamma'{{ [M' | Gamma]) 
+| get_here_LF M' Gamma'' => 
+  match eq_context_LF_dec Gamma' Gamma'' with
+    | left _ => get_here_LF ({{Delta ~> Gamma''}} M') (Gamma''++Delta)
+    | right _ => get_here_LF (}}Delta ~> Gamma'{{ [M' | Gamma'']) Gamma''
+  end
+| letdia_LF M' N => 
+  letdia_LF (}}Delta ~> Gamma'{{ [M' | Gamma]) (}}Delta ~> Gamma'{{ [N | Gamma])
+| letdia_get_LF M' N Gamma'' =>
+  match eq_context_LF_dec Gamma' Gamma'' with
+    | left _ => 
+      letdia_get_LF ({{Delta ~> Gamma''}} M') 
+                    (}}Delta ~> Gamma'{{ [N | Gamma]) (Gamma''++Delta)
+    | right _ =>  
+      letdia_get_LF (}}Delta ~> Gamma'{{ [M' | Gamma''])
+                    (}}Delta ~> Gamma'{{ [N | Gamma]) Gamma''
+  end
+end
+where " }} A ~> B {{ [ M | C ] " := (outer_term_weakening M C B A).
+
 (* TODO: ugly!!!... *)
 Lemma Weakening_general:
-forall G Gamma M A
+  forall G Gamma M A
   (HT: G |= Gamma |- M ::: A),
   (forall G' Delta Delta',
     permut G (G' & Delta) ->
-    G' & (Delta ++ Delta') |= Gamma |- M ::: A) /\ 
-  (forall Gamma', G |= Gamma ++ Gamma' |- M ::: A).
+    G' & (Delta ++ Delta') |= Gamma |- (}}Delta' ~> Delta{{ [M | Gamma]) ::: A) /\ 
+  (forall Gamma',
+    G |= Gamma ++ Gamma' |- ({{Gamma' ~> Gamma}}M) ::: A).
 intros;
-induction HT; split; intros.
+induction HT; split;
+intros; subst; simpl.
 (* hyp *)
 eauto using types_LF.
 constructor; generalize dependent v_n;
 induction Gamma; destruct v_n; intros;
-simpl in HT; try discriminate; simpl;
-[ | apply IHGamma]; assumption.
+try (apply Nth_nil_inv in HT; contradiction);
+apply Nth_app_l; assumption.
 (* lam *)
-constructor; eapply IHHT; eassumption.
-constructor; eapply IHHT; eassumption.
+constructor; eapply IHHT; eauto.
+constructor; eapply IHHT; eauto.
 (* appl *)
 econstructor; [eapply IHHT1| eapply IHHT2]; eauto.
 econstructor; [eapply IHHT1| eapply IHHT2]; eauto.
@@ -189,25 +324,25 @@ apply IHHT; permut_simpl.
 constructor; apply IHHT; assumption.
 constructor; apply IHHT; assumption.
 (* unbox_fetch 1 *)
-destruct (eq_context_dec Gamma Delta).
+destruct (eq_context_LF_dec Delta Gamma).
 (* = *)
-subst;
-apply t_unbox_fetch_LF with (Gamma:=Delta++Delta') (G:=G).
+subst.
+apply t_unbox_fetch_LF with (G:=G).
   apply IHHT.
   apply permut_app_l;
-  apply PermutLastSame with (elem:=Delta);
-  apply permut_trans with (l2:=G0); assumption.
+  apply PermutLastSame with (elem:=Gamma);
+  apply permut_trans with (l2:=G'); assumption.
 (* <> *)
-assert (exists G0, exists G1, G' = G0 & Gamma ++ G1).
+assert (exists G0, exists G1, G'0 = G0 & Gamma ++ G1).
   apply PermutationElementSplit_Neq with (G:=G) (G':=nil) (elem':=Delta).
-    assumption.
-    rew_app; apply permut_trans with (l2:=G0); assumption.
-destruct H1 as [GH]; destruct H1 as [GT]; subst G';
+    intro e; symmetry in e; contradiction.
+    rew_app; apply permut_trans with (l2:=G'); assumption.
+destruct H1 as [GH]; destruct H1 as [GT]; subst G'0.
 apply t_unbox_fetch_LF with (Gamma:=Gamma) (G:=GH ++ GT & (Delta ++ Delta')).
 apply BackgroundSubsetImpl with (G:= (GH ++ GT & Gamma') & (Delta ++ Delta')).
-  apply IHHT; permut_simpl;
-  apply PermutLastSame with (elem := Gamma);
-  apply permut_trans with (l2:=G0).
+  apply IHHT; permut_simpl.
+  apply PermutLastSame with (elem := Gamma).
+  apply permut_trans with (l2:=G').
     assumption.
     apply permut_trans with (l2:=(GH & Gamma ++ GT) & Delta).
       assumption.
@@ -222,18 +357,18 @@ apply t_unbox_fetch_LF with (G:=G) (Gamma:=Gamma).
 constructor; apply IHHT; assumption.
 constructor; apply IHHT; assumption.
 (* get_here 1 *)
-destruct (eq_context_dec Gamma Delta).
+destruct (eq_context_LF_dec Delta Gamma).
 (* = *)
 subst;
-apply t_get_here_LF with (Gamma:=Delta++Delta') (G:=G).
+apply t_get_here_LF with (Gamma:=Gamma++Delta') (G:=G).
   apply IHHT.
   apply permut_app_l;
-  apply PermutLastSame with (elem:=Delta);
+  apply PermutLastSame with (elem:=Gamma);
   apply permut_trans with (l2:=G0); assumption.
 (* <> *)
 assert (exists G0, exists G1, G' = G0 & Gamma ++ G1).
   apply PermutationElementSplit_Neq with (G:=G) (G':=nil) (elem':=Delta).
-    assumption.
+    intro e; symmetry in e; contradiction.
     rew_app; apply permut_trans with (l2:=G0); assumption.
 destruct H1 as [GH]; destruct H1 as [GT]; subst G';
 apply t_get_here_LF with (Gamma:=Gamma) (G:=GH ++ GT & (Delta ++ Delta')).
@@ -261,21 +396,21 @@ apply t_letdia_LF with (A:=A).
 apply IHHT1; assumption.
 apply IHHT2. 
 (* letdia_get 1 *)
-destruct (eq_context_dec Gamma Delta).
+destruct (eq_context_LF_dec Delta Gamma).
 (* = *)
 subst;
-apply t_letdia_get_LF with (A:=A)(Gamma:=Delta++Delta') (G:=G).
+apply t_letdia_get_LF with (A:=A)(Gamma:=Gamma++Delta') (G:=G).
 apply IHHT1; assumption.
-apply BackgroundSubsetImpl with (G:=((A::nil) :: G) & (Delta ++ Delta')).
+apply BackgroundSubsetImpl with (G:=((A::nil) :: G) & (Gamma ++ Delta')).
   apply IHHT2; permut_simpl.
   exists nil; permut_simpl.
 apply permut_app_l;
-apply PermutLastSame with (elem:=Delta); (* sad panda 8( *)
+apply PermutLastSame with (elem:=Gamma);
 apply permut_trans with (l2:=G0); assumption.
 (* <> *)
 assert (exists G0, exists G1, G' = G0 & Gamma ++ G1).
   apply PermutationElementSplit_Neq with (G:=G) (G':=nil) (elem':=Delta).
-    assumption.
+    intro e; symmetry in e; contradiction.
     rew_app; apply permut_trans with (l2:=G0); assumption.
 destruct H1 as [GH]; destruct H1 as [GT];
 subst G';
@@ -314,7 +449,7 @@ Qed.
 Lemma WeakeningBackgroundElem:
 forall G G' Delta Delta' Gamma M A
   (HT: G & Delta ++ G' |= Gamma |- M ::: A),
-  G & (Delta ++ Delta') ++ G' |= Gamma |- M ::: A.
+  G & (Delta ++ Delta') ++ G' |= Gamma |- }} Delta' ~> Delta{{ [M | Gamma] ::: A.
 intros.
 apply BackgroundSubsetImpl with (G:=(G++G') & (Delta ++ Delta')).
 assert (permut (G & Delta ++ G') ((G++G') & Delta)).
@@ -326,7 +461,7 @@ Qed.
 Lemma Weakening:
 forall G Gamma Gamma' M A
   (HT: G |= Gamma |- M ::: A),
-  G |= Gamma ++ Gamma' |- M ::: A.
+  G |= Gamma ++ Gamma' |- {{Gamma' ~> Gamma}}M ::: A.
 intros;
 eapply Weakening_general; eassumption.
 Qed.
@@ -337,10 +472,11 @@ forall G M A
     permut G G' -> 
     forall Ctx, Mem Ctx G' -> Ctx = nil)
   (HT: G |= nil |- M ::: A),
-  value_LF M \/ exists N, M |-> N.
+  value_LF M \/ exists N, (M, nil, G) |-> (N, nil, G).
 induction M; intros; eauto using value_LF.
 (* hyp *)
-inversion HT; destruct n; discriminate.
+inversion HT; destruct n;
+apply Nth_nil_inv in HT0; contradiction.
 (* appl *)
 right; inversion HT; subst;
 destruct (IHM1 (A0 ---> A) EmptyCtx HT1).
@@ -353,17 +489,19 @@ destruct (IHM ([*]A) EmptyCtx HT0).
   destruct H; eexists; constructor; eapply H.
 (* unbox_fetch *)
 right; inversion HT; subst.
-destruct (IHM ([*]A) EmptyCtx).
-assert (Gamma = nil).
-  apply EmptyCtx with (G':=G0 & Gamma).
+assert (c = nil).
+  apply EmptyCtx with (G':=G0 & c).
   apply permut_sym; assumption.
-  rewrite Mem_app_or_eq. right; rewrite Mem_cons_eq; left; reflexivity.
-subst. 
+  rewrite Mem_app_or_eq; right; rewrite Mem_cons_eq; left; reflexivity.
+subst; destruct (IHM ([*]A) EmptyCtx).
 apply BackgroundSubsetImpl with (G:=G0 & nil). 
 assumption.
 exists nil; rew_app; assumption.
 inversion H; subst; inversion HT0; subst; eexists; constructor.
-destruct H; eexists; constructor; eapply H.
+destruct H as [M'].
+exists (unbox_fetch_LF M' nil). 
+apply red_unbox_fetch_LF with (G':=G).
+assumption.
 (* here *)
 inversion HT; subst.
 destruct (IHM A0 EmptyCtx HT0).
@@ -371,41 +509,50 @@ left; apply val_here_LF; assumption.
 right; destruct H; exists (here_LF x); eauto using step_LF.
 (* get_here *)
 inversion HT; subst.
-destruct (IHM A0 EmptyCtx).
-assert (Gamma = nil).
-  apply EmptyCtx with (G' := G0 & Gamma).
+assert (c = nil).
+  apply EmptyCtx with (G' := G0 & c).
   apply permut_sym; assumption.
   rewrite Mem_app_or_eq; right;
   rewrite Mem_cons_eq; left; reflexivity.
-subst. 
+subst; destruct (IHM A0 EmptyCtx).
 apply BackgroundSubsetImpl with (G:=G0 & nil).
 assumption.
 exists nil; permut_simpl; assumption.
 left; econstructor; eassumption.
-right; destruct H; exists (get_here_LF x); eauto using step_LF.
+right; destruct H as [x]; exists (get_here_LF x nil);
+apply red_get_here_LF with (G':=G); assumption.
 (* letdia *)
 right; inversion HT; subst.
 destruct (IHM1 (<*>A0) EmptyCtx HT1).
 inversion H; subst; inversion HT1; subst.
-  exists [M//0]M2; eauto using step_LF.
-  exists [M//0]M2; eauto using step_LF.
+  exists ([M//0 | A0::nil][M2 | nil]);
+  apply red_letdia_here_LF; assumption.
+  exists ([M//0 | A0::nil][M2 | nil]);
+  apply red_letdia__get_here_LF; assumption.
 destruct H; exists (letdia_LF x M2); eauto using step_LF.
 (* letdia_get *)
 right; inversion HT; subst.
-destruct (IHM1 (<*>A0) EmptyCtx).
-assert (Gamma = nil).
-  apply EmptyCtx with (G' := G0 & Gamma).
+assert (c = nil).
+  apply EmptyCtx with (G' := G0 & c).
   apply permut_sym; assumption.
   rewrite Mem_app_or_eq; right;
   rewrite Mem_cons_eq; left; reflexivity.
-subst.
+subst; destruct (IHM1 (<*>A0) EmptyCtx).
 apply BackgroundSubsetImpl with (G:=G0 & nil).
 assumption.
 exists nil; permut_simpl; assumption.
 inversion H; subst; inversion HT1; subst.
-  exists [M//0]M2; eauto using step_LF.
-  exists [M//0]M2; eauto using step_LF.
-destruct H; exists (letdia_get_LF x M2); eauto using step_LF.
+  exists ([M//0 | A0::nil][M2 | nil]).
+  apply red_letdia_get__here_LF with (G':=G0&nil).
+    apply permut_app_l; assumption.
+    assumption.
+  exists ([M//0 | A0::nil][M2 | nil]).
+  apply red_letdia_get_get_here_LF with (G':=G0&nil).
+    apply permut_app_l; assumption.
+    assumption.
+destruct H as [x];
+exists (letdia_get_LF x M2 nil); 
+eauto using step_LF.
 Qed.
 
 (* Original formulations of modified typing rules can be reconstructed *)
@@ -421,7 +568,7 @@ Qed.
 Lemma test_unbox_fetch:
   forall G G' Gamma Gamma' M A,
     G & Gamma ++ G' |= Gamma' |- M ::: [*] A ->
-      G & Gamma' ++ G' |= Gamma |- unbox_fetch_LF M ::: A.
+      G & Gamma' ++ G' |= Gamma |- unbox_fetch_LF M Gamma' ::: A.
 intros;
 apply t_unbox_fetch_LF with (G:=G ++ G') (Gamma:=Gamma');
 [apply BackgroundSubsetImpl with (G:=G & Gamma ++ G') | permut_simpl];
@@ -431,7 +578,7 @@ Qed.
 Lemma test_get_here:
   forall G G' Gamma Gamma' M A,
     G & Gamma' ++ G' |= Gamma |- M ::: A ->
-      G & Gamma ++ G' |= Gamma' |- get_here_LF M ::: <*> A.
+      G & Gamma ++ G' |= Gamma' |- get_here_LF M Gamma ::: <*> A.
 intros;
 apply t_get_here_LF with (G:=G ++ G') (Gamma:=Gamma);
 [apply BackgroundSubsetImpl with (G:=G & Gamma' ++ G') | permut_simpl];
@@ -442,7 +589,7 @@ Lemma test_letdia_get:
   forall G G' Gamma Gamma' M N A B,
     G & Gamma' ++ G' |= Gamma |- M ::: <*>A ->
     (A::nil) :: G & Gamma ++ G' |= Gamma' |- N ::: B ->
-      G & Gamma ++ G' |= Gamma' |-  letdia_get_LF M N ::: B.
+      G & Gamma ++ G' |= Gamma' |-  letdia_get_LF M N Gamma ::: B.
 intros;
 apply t_letdia_get_LF with (A:=A) (Gamma:=Gamma) (G:=G ++ G');
 [ apply BackgroundSubsetImpl with (G:=G & Gamma' ++ G') |
