label-free/Syntax.v
@@ -1,4 +1,3 @@
-(* Types are exactly the same and should be shared between two languages *)
 Inductive ty_LF :=
 | tvar_LF: ty_LF
 | tarrow_LF: ty_LF -> ty_LF -> ty_LF
@@ -6,12 +5,13 @@ Inductive ty_LF :=
 | tdia_LF: ty_LF -> ty_LF
 .
 
-(* So are notations *)
 Notation " A '--->' B " := (tarrow_LF A B) (at level 30, right associativity) : label_free_is5_scope.
 Notation " '[*]' A " := (tbox_LF A) (at level 30) : label_free_is5_scope.
 Notation " '<*>' A " := (tdia_LF A) (at level 30) : label_free_is5_scope.
 
 Open Scope label_free_is5_scope.
+
+Definition Context_LF := list ty_LF.
 
 Inductive te_LF :=
 | hyp_LF: nat -> te_LF
@@ -19,11 +19,33 @@ Inductive te_LF :=
 | appl_LF: te_LF -> te_LF -> te_LF
 | box_LF: te_LF -> te_LF
 | unbox_LF: te_LF -> te_LF
-| unbox_fetch_LF: te_LF -> te_LF
+| unbox_fetch_LF: te_LF -> Context_LF -> te_LF
 | here_LF: te_LF -> te_LF
-| get_here_LF: te_LF -> te_LF
+| get_here_LF: te_LF -> Context_LF -> te_LF
 | letdia_LF: te_LF -> te_LF -> te_LF
-| letdia_get_LF: te_LF -> te_LF -> te_LF
+| letdia_get_LF: te_LF -> te_LF -> Context_LF -> te_LF
 .
+
+Theorem eq_ty_LF_dec:
+forall t1 t2: ty_LF, {t1 = t2} + {t1 <> t2}.
+intros; decide equality.
+Qed.
+
+Theorem eq_te_LF_dec:
+forall t1 t2: te_LF, {t1 = t2} + {t1 <> t2}.
+intros; decide equality.
+decide equality.
+decide equality.
+decide equality; decide equality.
+decide equality; decide equality.
+decide equality; decide equality.
+Qed.
+
+Theorem eq_context_LF_dec:
+forall c1 c2: Context_LF, {c1 = c2} + {c1 <> c2}.
+intros.
+decide equality.
+decide equality.
+Qed.
 
 Close Scope label_free_is5_scope.
